
# Unit 1.6

For every x, for every y, P(x, y)

p = the sum of two positive numbers is a positive number

P(x, y) = if (x > 0 and y > 0) then (x + y > 0)

# 1.6.1
# 1.6.3
# 1.6.4
# 1.6.5

for every x, there exists y, (x + y = 0) => true

# 1.6.7

domain ix Z+ x Z+
for every x, there exists a y, (x > y) => false (if x = 1)

# just all of 1.6 examples ig - it's just about chaining for everys and there exists.  

generalized De Morgan's Laws

~AxP(x) == Ex~P(x)

~ExP(x) == Ax~P(x)

~AxEyP(x, y) == Ex~EyP(x, y) == ExAy~P(x, y)

Ey~ExP(x, y) == EyAx~P(x, y)

~(x^2 > y + 1) == (x^2 >= y + 1) removed the negation by changing interior of proposition

EyAxP(x, y) = (x^2 >= y + 1) => there exists a y, where for every x, the proposition is satisfied. 

The picture you took in class
